src/simulation/ThreadsURA.v
@@ -1,6 +1,6 @@
 From sflib Require Import sflib.
 Require Import Coq.Classes.RelationClasses.
-From iris.algebra Require Import cmra updates functions lib.excl_auth.
+From iris.algebra Require Import cmra updates functions excl.
 
 From Fairness Require Import Axioms NatStructsLarge.
 From Fairness Require Import PCM.
@@ -8,15 +8,58 @@ From Fairness Require Import Mod.
 
 Set Implicit Arguments.
 
-(* Definition _thsRA {A: Type}: ucmra := Auth.t (Excl.t A). *)
-Definition thsRA {A: Type}: ucmra := (thread_id ==> (excl_authUR $ leibnizO A))%ra.
-(* Compute (URA.car (t:=_thsRA)). *)
-(* Global Instance thsRA {A: Type}: ucmra := Auth.t (@_thsRA A). *)
+Definition excl_authUR A : ucmra := (Auth.t $ optionUR $ exclR $ leibnizO A).
+
+Definition thsRA {A: Type}: ucmra := (thread_id ==> (excl_authUR A))%ra.
+
+Definition excl_auth_auth {A : Type} (a : A) : excl_authUR A :=
+  Auth.black (Some (Excl (a : leibnizO A))).
+Definition excl_auth_frag {A : Type} (a : A) : excl_authUR A :=
+  Auth.white (Some (Excl (a : leibnizO A))).
+
+Global Typeclasses Opaque excl_auth_auth excl_auth_frag.
+
+Global Instance: Params (@excl_auth_auth) 1 := {}.
+Global Instance: Params (@excl_auth_frag) 2 := {}.
+
+Notation "●E a" := (excl_auth_auth a) (at level 10).
+Notation "◯E a" := (excl_auth_frag a) (at level 10).
 
 Section THHAS.
 
-  Definition ae_white {A} (a: A) := ◯E (a : leibnizO A).
-  Definition ae_black {A} (a: A) := ●E (a : leibnizO A).
+  Definition ae_white {A} (a: A) : excl_authUR A  := ◯E a.
+  Definition ae_black {A} (a: A) : excl_authUR A := ●E a.
+
+  Lemma ae_white_black_agree {A} (a b : A) :
+    ✓ (ae_black a ⋅ ae_white b) → a = b.
+  Proof.
+    rewrite /ae_black /ae_white /excl_auth_auth /excl_auth_frag.
+    intros WF%Auth.auth_included%Excl_included.
+    by rewrite WF.
+  Qed.
+
+  Lemma ae_white_op_valid {A} (a a' : A) :
+    ✓ (ae_white a ⋅ ae_white a') → False.
+  Proof. done. Qed.
+
+  Lemma ae_black_white_valid {A} (a : A) :
+    ✓ (ae_black a ⋅ ae_white a).
+  Proof. done. Qed.
+
+  Lemma ae_black_white_extend {A} (a a' : A) (b : excl_authUR A) :
+    ✓ (ae_black a ⋅ ae_white a ⋅ b) →
+    ✓ (ae_black a' ⋅ ae_white a' ⋅ b).
+  Proof.
+    rewrite /ae_black /ae_white /excl_auth_auth /excl_auth_frag.
+    rewrite Auth.valid_unfold Auth.op_unfold.
+    simpl in *. intros WF.
+    rewrite left_id. rewrite left_id in WF. des_ifs.
+    destruct f as [[]|]; try done; simpl in *; des.
+    all: split; [|done].
+    all: rewrite -!Some_op; rewrite -!Some_op in WF.
+    all: rewrite Some_included in WF.
+    all: des; [inv WF|]; destruct WF as [[] ?]; inv H.
+  Qed.
 
   Definition th_has {A: Type} (tid: thread_id) (a: A): (@thsRA A) :=
     fun _tid => if (tid_dec _tid tid) then ae_white a else ε.
@@ -36,8 +79,8 @@ Section THHAS.
 
   Lemma th_has_disj {A: Type}: forall tid0 tid1 (a0 a1: A),
       ✓ (th_has tid0 a0 ⋅ th_has tid1 a1) -> tid0 <> tid1.
-  Proof. ii. clarify. specialize (H tid1). rewrite discrete_fun_lookup_op !th_has_hit in H. ss. eapply excl_auth_frag_op_valid,H. Qed.
+  Proof. ii. clarify. specialize (H tid1). rewrite discrete_fun_lookup_op !th_has_hit in H. ss. Qed.
 
 End THHAS.
 Notation "tid |-> a" := (th_has tid a) (at level 20).
-Global Opaque th_has.
+Global Opaque th_has ae_black ae_white.
